% Question 1

\begin{question}
    By considering \((r+1)^{3} - r^3\), derive the formula \(\sum_{r=1}^{n } r^2 = \frac{1}{6}n(n+1)(2n+1)\).
\end{question}

\begin{solution}
    Consider
    \begin{align*}
        (r+1)^{3} - r^3 &= r^3 + 3r^2 + 3r + 1 - r^3 \\
        &= 3r^2 + 3r + 1 \\
        \implies \sum_{r=1}^{n } \left[ (r+1)^{3} - r^3 \right] &= \sum_{r=1}^{n } \left[ 3r^2 + 3r + 1\right] \\
        \implies (n+1)^{3} - 1 &= \frac{3n (n+1)}{2}  + n + 3 \sum_{r=1}^{n } r^2 \\
        \implies 3 \sum_{r=1}^{n } r^2 &= n^3 + 3n^2 + 3n - \frac{3}{2} n^2 - \frac{3}{2}n - n \\
        &= n^3 + \frac{3}{2} n^2 + \frac{1}{2} n \\
        &= \frac{1}{2}n (2n^2 + 3n + 1) \\
        &= \frac{1}{2}n (2n+1)(n+1) \\
        \implies \sum_{r=1}^{n } r^2 &= \frac{1}{6} n(n+1)(2n+1 ) \qed
    \end{align*}

\end{solution}